new/proof/github_com/goose_lang/goose/testdata/examples/semantics.v
@@ -1,0 +1,114 @@
+From New.proof Require Import fmt.
+From New.proof.github_com.goose_lang Require Import primitive.
+From New.proof.github_com.goose_lang.primitive Require Import disk.
+From New.proof.github_com.goose_lang Require Import std.
+From New.proof Require Import log.
+From New.proof Require Import sync.
+From New.proof Require Import encoding.binary.
+From New.proof Require Import disk_prelude.
+From New.generatedproof.github_com.goose_lang.goose.testdata.examples Require Import unittest.
+From New.generatedproof Require Import fmt.
+From New.generatedproof.github_com.goose_lang.goose.testdata.examples
+  Require Import semantics.
+From New.proof Require Import proof_prelude.
+
+Unset Printing Records.
+
+Section wps.
+Context `{!heapGS Σ}.
+Context {sem : go.Semantics} {package_sem : semantics.Assumptions}.
+Local Set Default Proof Using "All".
+
+#[global] Instance : IsPkgInit (iProp Σ) semantics := define_is_pkg_init True%I.
+#[global] Instance : GetIsPkgInitWf (iProp Σ) semantics := build_get_is_pkg_init_wf.
+
+Definition test_fun_ok name :=
+  ∀ Φ, Φ #true -∗ WP @! name #() {{ Φ }}.
+
+Ltac semantics_auto :=
+  iIntros (Φ) "HΦ";
+  wp_func_call; wp_call;
+  try wp_auto;
+  try solve [ iExactEq "HΦ";
+              done ].
+
+Ltac wp_call_auto :=
+  (wp_func_call || wp_method_call); wp_call;
+  try wp_auto;
+  repeat rewrite -> decide_True by auto;
+  repeat rewrite -> decide_False by auto;
+  try wp_auto.
+
+Lemma wp_testU64ToU32 :
+  test_fun_ok semantics.testU64ToU32.
+Proof. semantics_auto. Qed.
+
+Lemma wp_testU32ToU64 :
+  test_fun_ok semantics.testU32ToU64.
+Proof. semantics_auto. Qed.
+
+Lemma wp_testU32Len :
+  test_fun_ok semantics.testU32Len.
+Proof.
+  semantics_auto.
+  wp_apply wp_slice_make2; [ word | ].
+  iIntros (?) "[Hs Hcap]".
+  wp_auto.
+  iDestruct (own_slice_len with "Hs") as %Hlen.
+  rewrite bool_decide_eq_true_2; [ wp_end | ].
+  rewrite length_replicate in Hlen.
+  word.
+Qed.
+
+Lemma wp_testU32NewtypeLen :
+  test_fun_ok semantics.testU32NewtypeLen.
+Proof.
+  semantics_auto.
+  wp_apply wp_slice_make2; [ word | ].
+  iIntros (?) "[Hs Hcap]".
+  wp_auto.
+  iDestruct (own_slice_len with "Hs") as %Hlen.
+  rewrite bool_decide_eq_true_2; [ wp_end | ].
+  rewrite length_replicate in Hlen.
+  word.
+Qed.
+
+Lemma wp_testUint32Untyped :
+  test_fun_ok semantics.testUint32Untyped.
+Proof. semantics_auto. Qed.
+
+Lemma wp_testPrimitiveTypesEqual :
+  test_fun_ok semantics.testPrimitiveTypesEqual.
+Proof.
+  semantics_auto.
+  repeat wp_call_auto.
+  wp_end.
+Qed.
+
+Lemma wp_testDefinedStrTypesEqual :
+  test_fun_ok semantics.testDefinedStrTypesEqual.
+Proof.
+  semantics_auto.
+  repeat wp_call_auto.
+  wp_end.
+Qed.
+
+Lemma wp_testListTypesEqual :
+  test_fun_ok semantics.testListTypesEqual.
+Proof.
+  semantics_auto.
+  repeat wp_call_auto.
+  wp_end.
+Qed.
+
+Lemma wp_testStructUpdates :
+  test_fun_ok semantics.testStructUpdates.
+Proof.
+  semantics_auto.
+  repeat (wp_call_auto || wp_call || wp_auto).
+  wp_alloc x1 as "H"; wp_auto.
+  repeat (wp_call_auto || wp_call || wp_auto).
+  wp_end.
+Qed.
+
+End wps.
